Definition of Algorithmic Typing and proof that it is deterministic

theories/AlgorithmicTyping.v
@@ -1,7 +1,7 @@
 (** * LogRel.AlgorithmicTyping: definition of algorithmic conversion and typing. *)
 From Coq Require Import ssrbool.
 From LogRel.AutoSubst Require Import core unscoped Ast Extra.
-From LogRel Require Import Utils BasicAst Notations Context NormalForms Weakening UntypedReduction GenericTyping DeclarativeTyping.
+From LogRel Require Import Utils BasicAst Notations LContexts Context NormalForms Weakening UntypedReduction GenericTyping DeclarativeTyping.
 
 Section Definitions.
 
@@ -12,182 +12,320 @@ Section Definitions.
 (** ** Conversion *)
 
   (** **** Conversion of types *)
-  Inductive ConvTypeAlg : context -> term -> term  -> Type :=
+  Inductive ConvTypeAlg (wl : wfLCon) : context -> term -> term  -> Type :=
     | typeConvRed {Γ A A' B B'} :
-      [A ⇒* A'] ->
-      [B ⇒* B'] ->
-      [Γ |- A' ≅h B'] ->
-      [Γ |- A ≅ B]
+      [A ⤳* A']< wl > ->
+      [B ⤳* B']< wl > ->
+      [Γ |- A' ≅h B']< wl > ->
+      [Γ |- A ≅ B]< wl >
   (** **** Conversion of types reduced to weak-head normal forms *)
-  with ConvTypeRedAlg : context -> term -> term -> Type :=
+  with ConvTypeRedAlg (wl : wfLCon) : context -> term -> term -> Type :=
     | typePiCongAlg {Γ A B A' B'} :
-      [ Γ |- A ≅ A'] ->
-      [ Γ ,, A |- B ≅ B'] ->
-      [ Γ |- tProd A B ≅h tProd A' B']
+      [ Γ |- A ≅ A']< wl > ->
+      [ Γ ,, A |- B ≅ B']< wl > ->
+      [ Γ |- tProd A B ≅h tProd A' B']< wl >
     | typeUnivConvAlg {Γ} :
-      [Γ |- U ≅h U]
+      [Γ |- U ≅h U]< wl >
     | typeNatConvAlg {Γ} :
-      [Γ |- tNat ≅h tNat]
+      [Γ |- tNat ≅h tNat]< wl >
+    | typeBoolConvAlg {Γ} :
+      [Γ |- tBool ≅h tBool]< wl >
     | typeEmptyConvAlg {Γ} :
-      [Γ |- tEmpty ≅h tEmpty]
+      [Γ |- tEmpty ≅h tEmpty]< wl >
+    | typeSigCongAlg {Γ A B A' B'} :
+      [ Γ |- A ≅ A']< wl > ->
+      [ Γ ,, A |- B ≅ B']< wl > ->
+      [ Γ |- tSig A B ≅h tSig A' B']< wl >
+    | typeIdCongAlg {Γ A A' x x' y y'} :
+      [ Γ |- A ≅ A']< wl > ->
+      [ Γ |- x ≅ x' : A]< wl > ->
+      [ Γ |- y ≅ y' : A]< wl > ->
+      [ Γ |- tId A x y ≅h tId A' x' y']< wl >
     | typeNeuConvAlg {Γ M N T} :
-      [ Γ |- M ~ N ▹ T] -> 
-      [ Γ |- M ≅h N]
+      [ Γ |- M ~ N ▹ T]< wl > -> 
+      [ Γ |- M ≅h N]< wl >
   (** **** Conversion of neutral terms *)
-  with ConvNeuAlg : context -> term -> term  -> term -> Type :=
+  with ConvNeuAlg (wl : wfLCon) : context -> term -> term  -> term -> Type :=
     | neuVarConvAlg {Γ n decl} :
       in_ctx Γ n decl ->
-      [Γ |- tRel n ~ tRel n ▹ decl]
+      [Γ |- tRel n ~ tRel n ▹ decl]< wl >
     | neuAppCongAlg {Γ m n t u A B} :
-      [ Γ |- m ~h n ▹ tProd A B ] ->
-      [ Γ |- t ≅ u : A ] ->
-      [ Γ |- tApp m t ~ tApp n u ▹ B[t..] ]
+      [ Γ |- m ~h n ▹ tProd A B ]< wl > ->
+      [ Γ |- t ≅ u : A ]< wl > ->
+      [ Γ |- tApp m t ~ tApp n u ▹ B[t..] ]< wl >
     | neuNatElimCong {Γ n n' P P' hz hz' hs hs'} :
     (** Here, we know by invariant that the inferred type has to be tNat,
     so there should be no need to check that, but with parameterized/indexed
     inductive we need to recover informations from the neutrals to construct
     the context for the predicate and the type of the branches. *)
-      [Γ |- n ~h n' ▹ tNat] ->
-      [Γ,, tNat |- P ≅ P'] ->
-      [Γ |- hz ≅ hz' : P[tZero..]] ->
-      [Γ |- hs ≅ hs' : elimSuccHypTy P] ->
-      [Γ |- tNatElim P hz hs n ~ tNatElim P' hz' hs' n' ▹ P[n..]]
+      [Γ |- n ~h n' ▹ tNat]< wl > ->
+      [Γ,, tNat |- P ≅ P']< wl > ->
+      [Γ |- hz ≅ hz' : P[tZero..]]< wl > ->
+      [Γ |- hs ≅ hs' : elimSuccHypTy P]< wl > ->
+      [Γ |- tNatElim P hz hs n ~ tNatElim P' hz' hs' n' ▹ P[n..]]< wl >
+    | neuBoolElimCong {Γ n n' P P' ht ht' hf hf'} :
+      [Γ |- n ~h n' ▹ tBool]< wl > ->
+      [Γ,, tBool |- P ≅ P']< wl > ->
+      [Γ |- ht ≅ ht' : P[tTrue..]]< wl > ->
+      [Γ |- hf ≅ hf' : P[tFalse..]]< wl > ->
+      [Γ |- tBoolElim P ht hf n ~ tBoolElim P' ht' hf' n' ▹ P[n..]]< wl >
     | neuEmptyElimCong {Γ P P' e e'} :
-      [Γ |- e ~h e' ▹ tEmpty] ->
-      [Γ ,, tEmpty |- P ≅ P'] ->
-      [Γ |- tEmptyElim P e ~ tEmptyElim P' e' ▹ P[e..]]
+      [Γ |- e ~h e' ▹ tEmpty]< wl > ->
+      [Γ ,, tEmpty |- P ≅ P']< wl > ->
+      [Γ |- tEmptyElim P e ~ tEmptyElim P' e' ▹ P[e..]]< wl >
+    | neuFstCongAlg {Γ m n A B} :
+      [ Γ |- m ~h n ▹ tSig A B ]< wl > ->
+      [ Γ |- tFst m ~ tFst n ▹ A ]< wl >
+    | neuSndCongAlg {Γ m n A B} :
+      [ Γ |- m ~h n ▹ tSig A B ]< wl > ->
+      [ Γ |- tSnd m ~ tSnd n ▹ B[(tFst m)..] ]< wl >
+    | neuIdEmlimCong {Γ A A' A'' x x' x'' P P' hr hr' y y' y'' e e'} :
+      [Γ |- e ~h e' ▹ tId A'' x'' y'']< wl > ->
+      (* [Γ |- A'' ]< wl > -> *)
+      (* [Γ |- A'' ≅ A]< wl > -> *)
+      (* [Γ |- x'' ◃ A]< wl > -> *)
+      (* [Γ |- x'' ≅ x : A]< wl > -> *)
+      (* [Γ |- y'' ◃ A]< wl > -> *)
+      (* [Γ |- y'' ≅ y : A]< wl > -> *)
+      [Γ |- A ≅ A']< wl > ->
+      [Γ |- x ≅ x' : A]< wl > ->
+      [Γ ,, A ,, tId A⟨@wk1 Γ A⟩ x⟨@wk1 Γ A⟩ (tRel 0) |- P ≅ P']< wl > ->
+      [Γ |- hr ≅ hr' : P[tRefl A x .: x..]]< wl > ->
+      [Γ |- y ≅ y' : A]< wl > ->
+      [Γ |- tIdElim A x P hr y e ~ tIdElim A' x' P' hr' y' e' ▹ P[e .: y..] ]< wl >
+    | neuAlphaCong {Γ n n' k} :
+      [Γ |- n ~ n' ▹ tNat]< wl > ->
+      [Γ |- tAlpha (nSucc k n) ~ tAlpha (nSucc k n') ▹ tBool]< wl >
   (** **** Conversion of neutral terms at a type reduced to weak-head normal form*)
-  with ConvNeuRedAlg : context -> term -> term -> term -> Type :=
+  with ConvNeuRedAlg (wl : wfLCon) : context -> term -> term -> term -> Type :=
     | neuConvRed {Γ m n A A'} :
-      [Γ |- m ~ n ▹ A] ->
-      [A ⇒* A'] ->
+      [Γ |- m ~ n ▹ A]< wl > ->
+      [A ⤳* A']< wl > ->
       isType A' ->
-      [Γ |- m ~h n ▹ A']
+      [Γ |- m ~h n ▹ A']< wl >
   (** **** Conversion of terms *)
-  with ConvTermAlg : context -> term -> term -> term -> Type :=
+  with ConvTermAlg (wl : wfLCon) : context -> term -> term -> term -> Type :=
     | termConvRed {Γ t t' u u' A A'} :
-      [A ⇒* A'] ->
-      [t ⇒* t'] ->
-      [u ⇒* u' ] ->
-      [Γ |- t' ≅h u' : A'] ->
-      [Γ |- t ≅ u : A]
+      [A ⤳* A']< wl > ->
+      [t ⤳* t']< wl > ->
+      [u ⤳* u' ]< wl > ->
+      [Γ |- t' ≅h u' : A']< wl > ->
+      [Γ |- t ≅ u : A]< wl >
+    | ϝtermConv_l {Γ n P ht hf t} {ne : not_in_LCon (pi1 wl) n} :
+      [Γ |- ht ≅ t : P[tTrue..]]< wl ,,l (ne, true) > ->
+      [Γ |- hf ≅ t : P[tFalse..]]< wl ,,l (ne, false) > ->
+      [Γ |- tBoolElim P ht hf (tAlpha (nat_to_term n)) ≅ t : P[(tAlpha (nat_to_term n))..]]< wl >
+    | ϝtermConv_r {Γ n P ht hf t} {ne : not_in_LCon (pi1 wl) n} :
+      [Γ |- t ≅ ht : P[tTrue..]]< wl ,,l (ne, true) > ->
+      [Γ |- t ≅ hf : P[tFalse..]]< wl ,,l (ne, false) > ->
+      [Γ |- t ≅ tBoolElim P ht hf (tAlpha (nat_to_term n)) : P[(tAlpha (nat_to_term n))..]]< wl >
   (** **** Conversion of terms reduced to a weak-head normal form at a reduced type *)
-  with ConvTermRedAlg : context -> term -> term -> term -> Type :=
+  with ConvTermRedAlg (wl : wfLCon) : context -> term -> term -> term -> Type :=
     | termPiCongAlg {Γ A B A' B'} :
-      [ Γ |- A ≅ A' : U] ->
-      [ Γ ,, A |- B ≅ B' : U] ->
-      [ Γ |- tProd A B ≅h tProd A' B' : U]
+      [ Γ |- A ≅ A' : U]< wl > ->
+      [ Γ ,, A |- B ≅ B' : U]< wl > ->
+      [ Γ |- tProd A B ≅h tProd A' B' : U]< wl >
     | termNatReflAlg {Γ} :
-      [Γ |- tNat ≅h tNat : U]
+      [Γ |- tNat ≅h tNat : U]< wl >
     | termZeroReflAlg {Γ} :
-      [Γ |- tZero ≅h tZero : tNat]
+      [Γ |- tZero ≅h tZero : tNat]< wl >
     | termSuccCongAlg {Γ t t'} :
-      [Γ |- t ≅ t' : tNat] ->
-      [Γ |- tSucc t ≅h tSucc t' : tNat]
+      [Γ |- t ≅ t' : tNat]< wl > ->
+      [Γ |- tSucc t ≅h tSucc t' : tNat]< wl >
+    | termBoolReflAlg {Γ} :
+      [Γ |- tBool ≅h tBool : U]< wl >
+    | termTrueReflAlg {Γ} :
+      [Γ |- tTrue ≅h tTrue : tBool]< wl >
+    | termFalseReflAlg {Γ} :
+      [Γ |- tFalse ≅h tFalse : tBool]< wl >
     | termEmptyReflAlg {Γ} :
-      [Γ |- tEmpty ≅h tEmpty : U]
+      [Γ |- tEmpty ≅h tEmpty : U]< wl >
     | termFunConvAlg {Γ : context} {f g A B} :
       isFun f ->
       isFun g ->
-      [ Γ,, A |- eta_expand f ≅ eta_expand g : B] -> 
-      [ Γ |- f ≅h g : tProd A B]
+      [ Γ,, A |- eta_expand f ≅ eta_expand g : B]< wl > -> 
+      [ Γ |- f ≅h g : tProd A B]< wl >
+    | termSigCongAlg {Γ A B A' B'} :
+      [ Γ |- A ≅ A' : U]< wl > ->
+      [ Γ ,, A |- B ≅ B' : U]< wl > ->
+      [ Γ |- tSig A B ≅h tSig A' B' : U]< wl >
+    | termPairConvAlg {Γ : context} {p q A B} :
+      whnf p ->
+      whnf q ->
+      [ Γ |- tFst p ≅ tFst q : A]< wl > -> 
+      [ Γ |- tSnd p ≅ tSnd q : B[(tFst p)..]]< wl > -> 
+      [ Γ |- p ≅h q : tSig A B]< wl >
+    | termIdCongAlg {Γ A A' x x' y y'} :
+      [Γ |- A ≅ A' : U]< wl > ->
+      [Γ |- x ≅ x' : A]< wl > ->
+      [Γ |- y ≅ y' : A]< wl > ->
+      [Γ |- tId A x y ≅h tId A' x' y' : U]< wl >
+    | termIdReflCong {Γ A A' A'' x x' y y'} :
+      [Γ |- A ≅ A']< wl > ->
+      [Γ |- x ≅ x' : A]< wl > ->
+      [Γ |- tRefl A x ≅h tRefl A' x' : tId A'' y y' ]< wl >
     | termNeuConvAlg {Γ m n T P} :
-      [Γ |- m ~ n ▹ T] ->
+      [Γ |- m ~ n ▹ T]< wl > ->
       isPosType P ->
-      [Γ |- m ≅h n : P]
+      [Γ |- m ≅h n : P]< wl >
 
-  where "[ Γ |- A ≅ B ]" := (ConvTypeAlg Γ A B)
-  and "[ Γ |- A ≅h B ]" := (ConvTypeRedAlg Γ A B)
-  and "[ Γ |- m ~ n ▹ T ]" := (ConvNeuAlg Γ T m n)
-  and "[ Γ |- m ~h n ▹ T ]" := (ConvNeuRedAlg Γ T m n)
-  and "[ Γ |- t ≅ u : T ]" := (ConvTermAlg Γ T t u)
-  and "[ Γ |- t ≅h u : T ]" := (ConvTermRedAlg Γ T t u)
-  and "[ t ⇒ t' ]" := (OneRedAlg t t')
-  and "[ t ⇒* t' ]" := (RedClosureAlg t t').
+  where "[ Γ |- A ≅ B ]< wl >" := (ConvTypeAlg wl Γ A B)
+  and "[ Γ |- A ≅h B ]< wl >" := (ConvTypeRedAlg wl Γ A B)
+  and "[ Γ |- m ~ n ▹ T ]< wl >" := (ConvNeuAlg wl Γ T m n)
+  and "[ Γ |- m ~h n ▹ T ]< wl >" := (ConvNeuRedAlg wl Γ T m n)
+  and "[ Γ |- t ≅ u : T ]< wl >" := (ConvTermAlg wl Γ T t u)
+  and "[ Γ |- t ≅h u : T ]< wl >" := (ConvTermRedAlg wl Γ T t u)
+  and "[ t ⤳ t' ]< wl >" := (@OneRedAlg wl t t')
+  and "[ t ⤳* t' ]< wl >" := (@RedClosureAlg wl t t').
 
 (** ** Typing *)
 
   (** **** Type well-formation *)
-  Inductive WfTypeAlg : context -> term -> Type :=
-    | wfTypeU Γ : [ Γ |- U ]
+  Inductive WfTypeAlg (wl : wfLCon) : context -> term -> Type :=
+    | wfTypeU Γ : [ Γ |- U ]< wl >
     | wfTypeProd {Γ A B} :
-      [Γ |- A ] ->
-      [Γ,, A |- B] ->
-      [Γ |- tProd A B]
+      [Γ |- A ]< wl > ->
+      [Γ,, A |- B]< wl > ->
+      [Γ |- tProd A B]< wl >
     | wfTypeNat {Γ} :
-      [Γ |- tNat]
+      [Γ |- tNat]< wl >
+    | wfTypeBool {Γ} :
+      [Γ |- tBool]< wl >
     | wfTypeEmpty {Γ} :
-        [Γ |- tEmpty]
+        [Γ |- tEmpty]< wl >
+    | wfTypeSig {Γ A B} :
+      [Γ |- A ]< wl > ->
+      [Γ,, A |- B]< wl > ->
+      [Γ |- tSig A B]< wl >
+    | wfTypeId {Γ A x y} :
+      [Γ |- A]< wl > ->
+      [Γ |- x ◃ A]< wl > ->
+      [Γ |- y ◃ A]< wl > ->
+      [Γ |- tId A x y]< wl >
     | wfTypeUniv {Γ A} :
-      [Γ |- A ◃ U] ->
-      [Γ |- A]
+      ~ isCanonical A ->
+      [Γ |- A ▹h U]< wl > ->
+      [Γ |- A]< wl >
   (** **** Type inference *)
-  with InferAlg : context -> term -> term -> Type :=
+  with InferAlg (wl : wfLCon) : context -> term -> term -> Type :=
     | infVar {Γ n decl} :
       in_ctx Γ n decl ->
-      [Γ |- tRel n ▹ decl]
+      [Γ |- tRel n ▹ decl]< wl >
     | infProd {Γ} {A B} :
-      [ Γ |- A ▹h U] -> 
-      [Γ ,, (A) |- B ▹h U ] ->
-      [ Γ |- tProd A B ▹ U ]
+      [ Γ |- A ▹h U]< wl > -> 
+      [Γ ,, A |- B ▹h U ]< wl > ->
+      [ Γ |- tProd A B ▹ U ]< wl >
     | infLam {Γ} {A B t} :
-      [ Γ |- A] ->
-      [ Γ ,, A |- t ▹ B ] -> 
-      [ Γ |- tLambda A t ▹ tProd A B]
+      [ Γ |- A]< wl > ->
+      [ Γ ,, A |- t ▹ B ]< wl > -> 
+      [ Γ |- tLambda A t ▹ tProd A B]< wl >
     | infApp {Γ} {f a A B} :
-      [ Γ |- f ▹h tProd A B ] -> 
-      [ Γ |- a ◃ A ] -> 
-      [ Γ |- tApp f a ▹ B[a..] ]
+      [ Γ |- f ▹h tProd A B ]< wl > -> 
+      [ Γ |- a ◃ A ]< wl > -> 
+      [ Γ |- tApp f a ▹ B[a..] ]< wl >
     | infNat {Γ} :
-      [Γ |- tNat ▹ U]
+      [Γ |- tNat ▹ U]< wl >
     | infZero {Γ} :
-      [Γ |- tZero ▹ tNat]
+      [Γ |- tZero ▹ tNat]< wl >
     | infSucc {Γ t} :
-      [Γ |- t ▹h tNat] ->
-      [Γ |- tSucc t ▹ tNat]
+      [Γ |- t ▹h tNat]< wl > ->
+      [Γ |- tSucc t ▹ tNat]< wl >
     | infNatElim {Γ P hz hs n} :
-      [Γ |- n ▹h tNat] ->
-      [Γ,, tNat |- P] ->
-      [Γ |- hz ◃ P[tZero..]] ->
-      [Γ |- hs ◃ elimSuccHypTy P] ->
-      [Γ |- tNatElim P hz hs n ▹ P[n..]]
+      [Γ |- n ▹h tNat]< wl > ->
+      [Γ,, tNat |- P]< wl > ->
+      [Γ |- hz ◃ P[tZero..]]< wl > ->
+      [Γ |- hs ◃ elimSuccHypTy P]< wl > ->
+      [Γ |- tNatElim P hz hs n ▹ P[n..]]< wl >
+    | infBool {Γ} :
+      [Γ |- tBool ▹ U]< wl >
+    | infTrue {Γ} :
+      [Γ |- tTrue ▹ tBool]< wl >
+    | infFalse {Γ} :
+      [Γ |- tFalse ▹ tBool]< wl >
+    | infAlpha {Γ t} :
+      [Γ |- t ▹h tNat]< wl > ->
+      [Γ |- tAlpha t ▹ tBool]< wl >
+    | infBoolElim {Γ P ht hf n} :
+      [Γ |- n ▹h tBool]< wl > ->
+      [Γ,, tBool |- P]< wl > ->
+      [Γ |- ht ◃ P[tTrue..]]< wl > ->
+      [Γ |- hf ◃ P[tFalse..]]< wl > ->
+      [Γ |- tBoolElim P ht hf n ▹ P[n..]]< wl >
     | infEmpty {Γ} :
-      [Γ |- tEmpty ▹ U]
+      [Γ |- tEmpty ▹ U]< wl >
     | infEmptyElim {Γ P e} :
-      [Γ |- e ▹h tEmpty] ->
-      [Γ ,, tEmpty |- P ] ->
-      [Γ |- tEmptyElim P e ▹ P[e..]]
+      [Γ |- e ▹h tEmpty]< wl > ->
+      [Γ ,, tEmpty |- P ]< wl > ->
+      [Γ |- tEmptyElim P e ▹ P[e..]]< wl >
+    | infSig {Γ} {A B} :
+      [ Γ |- A ▹h U]< wl > -> 
+      [Γ ,, A |- B ▹h U ]< wl > ->
+      [ Γ |- tSig A B ▹ U ]< wl >
+    | infPair {Γ A B a b} :
+      [ Γ |- A]< wl > -> 
+      [Γ ,, A |- B]< wl > ->
+      [Γ |- a ◃ A]< wl > ->
+      [Γ |- b ◃ B[a..]]< wl > ->
+      [Γ |- tPair A B a b ▹ tSig A B]< wl >
+    | infFst {Γ A B p} :
+      [Γ |- p ▹h tSig A B]< wl > ->
+      [Γ |- tFst p ▹ A]< wl >
+    | infSnd {Γ A B p} :
+      [Γ |- p ▹h tSig A B]< wl > ->
+      [Γ |- tSnd p ▹ B[(tFst p)..]]< wl >
+    | infId {Γ A x y} :
+      [Γ |- A ▹h U]< wl > ->
+      [Γ |- x ◃ A]< wl > ->
+      [Γ |- y ◃ A]< wl > ->
+      [Γ |- tId A x y ▹ U]< wl >
+    | infRefl {Γ A x} :
+      [Γ |- A]< wl > ->
+      [Γ |- x ◃ A]< wl > ->
+      [Γ |- tRefl A x ▹ tId A x x]< wl >
+    | infIdElim {Γ A x P hr y e} :
+      [Γ |- A]< wl > ->
+      [Γ |- x ◃ A]< wl > ->
+      [Γ,, A,, tId A⟨@wk1 Γ A⟩ x⟨@wk1 Γ A⟩ (tRel 0) |- P]< wl > ->
+      [Γ |- hr ◃ P[tRefl A x .: x..]]< wl > ->
+      [Γ |- y ◃ A]< wl > ->
+      [Γ |- e ◃ tId A x y]< wl > ->
+      [Γ |- tIdElim A x P hr y e ▹ P[e .: y..]]< wl >
   (** **** Inference of a type reduced to weak-head normal form*)
-  with InferRedAlg : context -> term -> term -> Type :=
+  with InferRedAlg (wl : wfLCon) : context -> term -> term -> Type :=
     | infRed {Γ t A A'} :
-      [Γ |- t ▹ A ] ->
-      [ A ⇒* A'] ->
-      [Γ |- t ▹h A']
+      [Γ |- t ▹ A ]< wl > ->
+      [ A ⤳* A']< wl > ->
+      [Γ |- t ▹h A']< wl >
   (** **** Type-checking *)
-  with CheckAlg : context -> term -> term -> Type :=
+  with CheckAlg (wl : wfLCon) : context -> term -> term -> Type :=
     | checkConv {Γ t A A'} :
-      [ Γ |- t ▹ A ] -> 
-      [ Γ |- A ≅ A'] -> 
-      [ Γ |- t ◃ A' ]
+      [ Γ |- t ▹ A ]< wl > -> 
+      [ Γ |- A ≅ A']< wl > -> 
+      [ Γ |- t ◃ A' ]< wl >
 
-  where "[ Γ |- A ]" := (WfTypeAlg Γ A)
-  and "[ Γ |- t ▹ T ]" := (InferAlg Γ T t)
-  and "[ Γ |- t ▹h T ]" := (InferRedAlg Γ T t)
-  and "[ Γ |- t ◃ T ]" := (CheckAlg Γ T t).
+  where "[ Γ |- A ]< wl >" := (WfTypeAlg wl Γ A)
+  and "[ Γ |- t ▹ T ]< wl >" := (InferAlg wl Γ T t)
+  and "[ Γ |- t ▹h T ]< wl >" := (InferRedAlg wl Γ T t)
+  and "[ Γ |- t ◃ T ]< wl >" := (CheckAlg wl Γ T t).
 
   (** Context well-formation *)
-  Inductive WfContextAlg : context -> Type :=
-  | conNilAlg : [|- ε]
+  Inductive WfContextAlg (wl : wfLCon) : context -> Type :=
+  | conNilAlg : [|- ε]< wl >
   | conConsAlg {Γ A} :
-    [|- Γ] ->
-    [ Γ |- A] ->
-    [|- Γ,, A]
-  where "[ |- Γ ]" := (WfContextAlg Γ).
+    [|- Γ]< wl > ->
+    [ Γ |- A]< wl > ->
+    [|- Γ,, A]< wl >
+  where "[ |- Γ ]< wl >" := (WfContextAlg wl Γ).
 
 End Definitions.
 
 (** ** Instances *)
 Module AlgorithmicTypingData.
+
+  Definition al : tag.
+  Proof.
+  constructor.
+  Qed.
 
   #[export] Instance WfContext_Algo : WfContext al := WfContextAlg.
   #[export] Instance WfType_Algo : WfType al := WfTypeAlg.
@@ -240,7 +378,7 @@ Scheme
     Minimality for WfTypeAlg Sort Type with
     Minimality for InferAlg Sort Type with
     Minimality for InferRedAlg Sort Type with
-    Minimality for CheckAlg Sort Type.
+      Minimality for CheckAlg Sort Type.
 
 Combined Scheme _AlgoConvInduction from
     ConvTypeAlg_rect_nodep,
@@ -273,7 +411,7 @@ Lemma AlgoConvInduction : AlgoConvInductionType.
 Proof.
   intros PTyEq PTyRedEq PNeEq PNeRedEq PTmEq PTmRedEq **.
   pose proof (_AlgoConvInduction PTyEq PTyRedEq PNeEq PNeRedEq PTmEq PTmRedEq) as H.
-  destruct H as [?[?[?[?[?]]]]] ; cycle -1.
+  destruct H with (wl := wl) as [?[?[?[?[?]]]]] ; cycle -1.
   1: by_prod_splitter.
   all: assumption.
 Qed.
@@ -293,8 +431,8 @@ Let AlgoTypingInductionType :=
 
 Lemma AlgoTypingInduction : AlgoTypingInductionType.
 Proof.
-  intros PTy PInf PInfRed PCheck **.
-  pose proof (_AlgoTypingInduction PTy PInf PInfRed PCheck) as H.
+  intros wl PTy PInf PInfRed PCheck **.
+  pose proof (_AlgoTypingInduction wl PTy PInf PInfRed PCheck) as H.
   destruct H as [?[?[?]]] ; cycle -1.
   1: by_prod_splitter.
   all: assumption.
@@ -322,25 +460,25 @@ Arguments AlgoTypingInductionConcl PTy PInf PInfRed PCheck : rename.
 Section TypingWk.
   Import AlgorithmicTypingData.
   
-  Let PTyEq (Γ : context) (A B : term) := forall Δ (ρ : Δ ≤ Γ),
-    [Δ |- A⟨ρ⟩ ≅ B⟨ρ⟩].
-  Let PTyRedEq (Γ : context) (A B : term) := forall Δ (ρ : Δ ≤ Γ),
-      [Δ |- A⟨ρ⟩ ≅h B⟨ρ⟩].
-  Let PNeEq (Γ : context) (A t u : term) := forall Δ (ρ : Δ ≤ Γ),
-    [Δ |- t⟨ρ⟩ ~ u⟨ρ⟩ ▹ A⟨ρ⟩].
-  Let PNeRedEq (Γ : context) (A t u : term) := forall Δ (ρ : Δ ≤ Γ),
-    [Δ |- t⟨ρ⟩ ~h u⟨ρ⟩ ▹ A⟨ρ⟩].
-  Let PTmEq (Γ : context) (A t u : term) := forall Δ (ρ : Δ ≤ Γ),
-    [Δ |- t⟨ρ⟩ ≅ u⟨ρ⟩ : A⟨ρ⟩].
-  Let PTmRedEq (Γ : context) (A t u : term) := forall Δ (ρ : Δ ≤ Γ),
-      [Δ |- t⟨ρ⟩ ≅h u⟨ρ⟩ : A⟨ρ⟩].
+  Let PTyEq (wl : wfLCon) (Γ : context) (A B : term) := forall Δ (ρ : Δ ≤ Γ),
+    [Δ |- A⟨ρ⟩ ≅ B⟨ρ⟩]< wl >.
+  Let PTyRedEq (wl : wfLCon) (Γ : context) (A B : term) := forall Δ (ρ : Δ ≤ Γ),
+      [Δ |- A⟨ρ⟩ ≅h B⟨ρ⟩]< wl >.
+  Let PNeEq (wl : wfLCon) (Γ : context) (A t u : term) := forall Δ (ρ : Δ ≤ Γ),
+    [Δ |- t⟨ρ⟩ ~ u⟨ρ⟩ ▹ A⟨ρ⟩]< wl >.
+  Let PNeRedEq (wl : wfLCon) (Γ : context) (A t u : term) := forall Δ (ρ : Δ ≤ Γ),
+    [Δ |- t⟨ρ⟩ ~h u⟨ρ⟩ ▹ A⟨ρ⟩]< wl >.
+  Let PTmEq (wl : wfLCon) (Γ : context) (A t u : term) := forall Δ (ρ : Δ ≤ Γ),
+    [Δ |- t⟨ρ⟩ ≅ u⟨ρ⟩ : A⟨ρ⟩]< wl >.
+  Let PTmRedEq (wl : wfLCon) (Γ : context) (A t u : term) := forall Δ (ρ : Δ ≤ Γ),
+      [Δ |- t⟨ρ⟩ ≅h u⟨ρ⟩ : A⟨ρ⟩]< wl >.
 
-  Theorem algo_conv_wk :
+  Theorem algo_conv_wk (wl : wfLCon) :
     AlgoConvInductionConcl PTyEq PTyRedEq
-      PNeEq PNeRedEq PTmEq PTmRedEq.
+      PNeEq PNeRedEq PTmEq PTmRedEq wl.
   Proof.
     subst PTyEq PTyRedEq PNeEq PNeRedEq PTmEq PTmRedEq.
-    apply AlgoConvInduction.
+    apply AlgoConvInduction ; clear wl.
     - intros.
       econstructor.
       all: eauto using credalg_wk.
@@ -355,7 +493,14 @@ Section TypingWk.
     - intros.
       now econstructor.
     - intros.
-      now econstructor.  
+      now econstructor.
+    - intros * ??? IHB ? *; do 2 rewrite <- wk_sig.
+      econstructor.
+      1: eauto.
+      now eapply IHB.
+    - intros; now econstructor.
+    - intros.
+      now econstructor.
     - intros * ? ? ?.
       eapply convne_meta_conv.
       1: econstructor ; eauto using in_ctx_wk.
@@ -383,22 +528,72 @@ Section TypingWk.
         * reflexivity.
       + now bsimpl.
       + now bsimpl.
+    - intros * ? IHn ? IHP ? IHt ? IHf *.
+      cbn.
+      eapply convne_meta_conv ; [econstructor|..] ; refold.
+      + eauto.
+      + now eapply (IHP _ (wk_up tBool ρ)).
+      + eapply convtm_meta_conv.
+        * eapply IHt.
+        * now bsimpl.
+        * reflexivity.
+      + eapply convtm_meta_conv.
+        * eapply IHf.
+        * now bsimpl.
+        * reflexivity.
+      + now bsimpl.
+      + now bsimpl.
     - intros * ? IHe ? IHP *.
       cbn.
       eapply convne_meta_conv ; [econstructor|..] ; refold.
       + eauto.
       + now eapply (IHP _ (wk_up tEmpty ρ)).
       + now bsimpl.
-      + now bsimpl. 
+      + now bsimpl.
+    - intros * ? IH *; cbn.
+      econstructor; now eapply IH.
+    - intros ???? A? ? IH *; cbn.
+      rewrite (subst_ren_wk_up (A:=A)).
+      econstructor; now eapply IH.
+    - intros * ? IHe (*?? ?? ??*) ?? ?? ? IHp **; erewrite <-2!wk_idElim, subst_ren_wk_up2.
+      econstructor; eauto.
+      + rewrite 2!(wk_up_wk1 ρ).
+        eapply IHp; constructor; tea.
+      + rewrite wk_refl, <- subst_ren_wk_up2; eauto.
+    - intros.
+      cbn ; do 2 rewrite nSucc_ren.
+      now econstructor.
     - intros.
       econstructor.
       + eauto.
       + eauto using credalg_wk.
-      + now eapply isType_ren. 
+      + gen_typing. 
     - intros.
       econstructor.
       1-3: eauto using credalg_wk.
       now eauto.
+    - intros * ? Ht ? Hf *.
+      cbn ; unfold nat_to_term ; rewrite nSucc_ren ; cbn.
+      rewrite (subst_ren_wk_up (A := tBool)) ; cbn ; rewrite nSucc_ren ; cbn.
+      change (nSucc n tZero) with (nat_to_term n).
+      unshelve eapply ϝtermConv_l ; [assumption | ..].
+      + change tTrue with (tTrue⟨ρ⟩).
+        rewrite <- (wk_up_ren_on _ _ _ tBool), <- subst_ren_wk_up.
+        now eapply Ht.
+      + change tFalse with (tFalse⟨ρ⟩).
+        rewrite <- (wk_up_ren_on _ _ _ tBool), <- subst_ren_wk_up.
+        now eapply Hf.
+    - intros * ? Ht ? Hf *.
+      cbn ; unfold nat_to_term ; rewrite nSucc_ren ; cbn.
+      rewrite (subst_ren_wk_up (A := tBool)) ; cbn ; rewrite nSucc_ren ; cbn.
+      change (nSucc n tZero) with (nat_to_term n).
+      unshelve eapply ϝtermConv_r ; [assumption | ..].
+      + change tTrue with (tTrue⟨ρ⟩).
+        rewrite <- (wk_up_ren_on _ _ _ tBool), <- subst_ren_wk_up.
+        now eapply Ht.
+      + change tFalse with (tFalse⟨ρ⟩).
+        rewrite <- (wk_up_ren_on _ _ _ tBool), <- subst_ren_wk_up.
+        now eapply Hf.
     - intros * ? ? ? IHB ? ?.
       cbn.
       econstructor.
@@ -408,31 +603,47 @@ Section TypingWk.
     - now econstructor.
     - now econstructor.
     - now econstructor.
+    - now econstructor.
+    - now econstructor.
+    - now econstructor.
     - intros * ? ? ? IH ? ?.
       cbn.
       econstructor.
-      1-2: now eauto using isFun_ren.
+      1-2: gen_typing.
       specialize IH with(ρ := wk_up _ ρ).
       cbn in *.
-      asimpl.
-      repeat (rewrite renRen_term in IH).
+      assert (eq: forall t, t⟨ρ⟩⟨↑⟩ = t⟨↑⟩⟨up_ren ρ⟩) by now asimpl.
+      do 2 rewrite eq.
       apply IH.
+    - intros * ??? IHB *. 
+      do 2 rewrite <- wk_sig.
+      econstructor.
+      1: now eauto.
+      now eapply IHB.
+    - intros * ??? IHfst ? IHsnd *.
+      rewrite <- wk_sig.
+      econstructor.
+      1,2: gen_typing.
+      1: eauto.
+      rewrite wk_fst, <- subst_ren_wk_up; eauto.
+    - intros; econstructor; eauto.
+    - intros; econstructor; eauto.
     - intros.
       econstructor.
       + eauto.
       + eauto using isPosType_ren.
   Qed.
 
-  Let PTy (Γ : context) (A : term) := forall Δ (ρ : Δ ≤ Γ), [Δ |- A⟨ρ⟩].
-  Let PInf (Γ : context) (A t : term) := forall Δ (ρ : Δ ≤ Γ),
-    [Δ |- t⟨ρ⟩ ▹ A⟨ρ⟩].
-  Let PInfRed (Γ : context) (A t : term) := forall Δ (ρ : Δ ≤ Γ),
-    [Δ |- t⟨ρ⟩ ▹h A⟨ρ⟩].
-  Let PCheck (Γ : context) (A t : term) := forall Δ (ρ : Δ ≤ Γ),
-  [Δ |- t⟨ρ⟩ ◃ A⟨ρ⟩].
-
-  Theorem algo_typing_wk :
-    AlgoTypingInductionConcl PTy PInf PInfRed PCheck.
+  Let PTy (wl : wfLCon) (Γ : context) (A : term) := forall Δ (ρ : Δ ≤ Γ), [Δ |- A⟨ρ⟩]< wl >.
+  Let PInf (wl : wfLCon) (Γ : context) (A t : term) := forall Δ (ρ : Δ ≤ Γ),
+    [Δ |- t⟨ρ⟩ ▹ A⟨ρ⟩]< wl >.
+  Let PInfRed (wl : wfLCon) (Γ : context) (A t : term) := forall Δ (ρ : Δ ≤ Γ),
+    [Δ |- t⟨ρ⟩ ▹h A⟨ρ⟩]< wl >.
+  Let PCheck (wl : wfLCon) (Γ : context) (A t : term) := forall Δ (ρ : Δ ≤ Γ),
+  [Δ |- t⟨ρ⟩ ◃ A⟨ρ⟩]< wl >.
+About AlgoTypingInductionConcl.
+  Theorem algo_typing_wk (wl : wfLCon) :
+    AlgoTypingInductionConcl wl (PTy wl) (PInf wl) (PInfRed wl) (PCheck wl).
   Proof.
     subst PTy PInf PInfRed PCheck.
     apply AlgoTypingInduction.
@@ -446,6 +657,15 @@ Section TypingWk.
       now econstructor.
     - now constructor.
     - now constructor.
+    - intros * ? ? ? IHB **.
+      rewrite <-wk_sig.
+      econstructor.
+      + now eauto.
+      + now eapply IHB.
+    - intros; rewrite <- wk_Id; econstructor; eauto.
+    - constructor.
+      + now intros ?%isCanonical_ren.
+      + eauto. 
     - intros.
       eapply typing_meta_conv.
       + now econstructor ; eapply in_ctx_wk.
@@ -482,6 +702,24 @@ Section TypingWk.
         unfold elimSuccHypTy.
         now bsimpl.
       + now bsimpl.
+    - now econstructor.
+    - now econstructor.
+    - now econstructor.
+    - intros ; cbn.
+      now econstructor.
+    - intros * ? IHn ? IHP ? IHt ? IHf *.
+      cbn in *.
+      eapply typing_meta_conv.
+      1: econstructor.
+      + eauto.
+      + eapply IHP with (ρ := wk_up _ ρ).
+      + eapply typing_meta_conv.
+        1: eapply IHt.
+        now bsimpl.
+      + eapply typing_meta_conv.
+        1: eapply IHf.
+        now bsimpl.
+      + now bsimpl.
     - intros.
       now econstructor.
     - intros * ? IHe ? IHP *.
@@ -490,7 +728,26 @@ Section TypingWk.
       1: econstructor.
       + eauto.
       + eapply IHP with (ρ := wk_up _ ρ).
-      + now bsimpl.        
+      + now bsimpl. 
+    - intros * ??? IHB *.
+      rewrite <- wk_sig.
+      econstructor; eauto.
+    - intros * ???????? *.
+      rewrite <- wk_pair, <-wk_sig.
+      econstructor.
+      1-3: now eauto.
+      rewrite <- subst_ren_wk_up; eauto.
+    - intros * ?? *.
+      rewrite <- wk_fst; now econstructor.
+    - intros ? A ?? ? IH *.
+      rewrite <- wk_snd, (subst_ren_wk_up (A:=A)).
+      econstructor.
+      now eapply IH.
+    - intros; rewrite <- wk_Id; econstructor; eauto.
+    - intros; rewrite <- wk_refl; econstructor; eauto.
+    - intros; erewrite <- wk_idElim, subst_ren_wk_up2; econstructor; eauto.
+      + rewrite 2!(wk_up_wk1 ρ); eauto.
+      + rewrite wk_refl, <- subst_ren_wk_up2; eauto.
     - intros.
       econstructor.
       + eauto.
@@ -501,13 +758,14 @@ Section TypingWk.
       + now eapply algo_conv_wk.
   Qed.
 
-  Corollary algo_conv_shift : AlgoConvInductionConcl
-      (fun (Γ : context) (A B : term) => forall T, [Γ,, T |- A⟨↑⟩ ≅ B⟨↑⟩])
-      (fun (Γ : context) (A B : term) => forall T, [Γ,, T |- A⟨↑⟩ ≅h B⟨↑⟩])
-      (fun (Γ : context) (A m n : term) => forall T, [Γ,, T |- m⟨↑⟩ ~ n⟨↑⟩ ▹ A⟨↑⟩])
-      (fun (Γ : context) (A m n : term) => forall T, [Γ,, T |- m⟨↑⟩ ~h n⟨↑⟩ ▹ A⟨↑⟩])
-      (fun (Γ : context) (A t u : term) => forall T, [Γ,, T |- t⟨↑⟩ ≅ u⟨↑⟩ : A⟨↑⟩])
-      (fun (Γ : context) (A t u : term) => forall T, [Γ,, T |- t⟨↑⟩ ≅h u⟨↑⟩ : A⟨↑⟩]).
+  Corollary algo_conv_shift (wl : wfLCon) : AlgoConvInductionConcl
+      (fun (wl : wfLCon) (Γ : context) (A B : term) => forall T, [Γ,, T |- A⟨↑⟩ ≅ B⟨↑⟩]< wl >)
+      (fun (wl : wfLCon) (Γ : context) (A B : term) => forall T, [Γ,, T |- A⟨↑⟩ ≅h B⟨↑⟩]< wl >)
+      (fun (wl : wfLCon) (Γ : context) (A m n : term) => forall T, [Γ,, T |- m⟨↑⟩ ~ n⟨↑⟩ ▹ A⟨↑⟩]< wl >)
+      (fun (wl : wfLCon) (Γ : context) (A m n : term) => forall T, [Γ,, T |- m⟨↑⟩ ~h n⟨↑⟩ ▹ A⟨↑⟩]< wl >)
+      (fun (wl : wfLCon) (Γ : context) (A t u : term) => forall T, [Γ,, T |- t⟨↑⟩ ≅ u⟨↑⟩ : A⟨↑⟩]< wl >)
+      (fun (wl : wfLCon) (Γ : context) (A t u : term) => forall T, [Γ,, T |- t⟨↑⟩ ≅h u⟨↑⟩ : A⟨↑⟩]< wl >)
+  wl.
   Proof.
     red.
     repeat match goal with |- _ × _ => split end.
@@ -518,11 +776,11 @@ Section TypingWk.
     all: now eapply Hty.
   Qed.
 
-  Corollary algo_typing_shift : AlgoTypingInductionConcl
-  (fun (Γ : context) (A : term) => forall T, [Γ,, T |- A⟨↑⟩])
-  (fun (Γ : context) (A t : term) => forall T, [Γ,, T |- t⟨↑⟩ ▹ A⟨↑⟩])
-  (fun (Γ : context) (A t : term) => forall T, [Γ,, T |- t⟨↑⟩ ▹h A⟨↑⟩])
-  (fun (Γ : context) (A t : term) => forall T, [Γ,, T |- t⟨↑⟩ ◃ A⟨↑⟩]).
+  Corollary algo_typing_shift (wl : wfLCon) : AlgoTypingInductionConcl wl
+  (fun  (Γ : context) (A : term) => forall T, [Γ,, T |- A⟨↑⟩]< wl >)
+  (fun  (Γ : context) (A t : term) => forall T, [Γ,, T |- t⟨↑⟩ ▹ A⟨↑⟩]< wl >)
+  (fun  (Γ : context) (A t : term) => forall T, [Γ,, T |- t⟨↑⟩ ▹h A⟨↑⟩]< wl >)
+  (fun  (Γ : context) (A t : term) => forall T, [Γ,, T |- t⟨↑⟩ ◃ A⟨↑⟩]< wl >).
   Proof.
   red.
   repeat match goal with |- _ × _ => split end.
@@ -541,24 +799,150 @@ End TypingWk.
 indeed imply that the relevant arguments are such weak-head normal forms/neutrals. *)
 Section AlgTypingWh.
 
-  Let PTyEq (Γ : context) (A B : term) := True.
-  Let PTyRedEq (Γ : context) (A B : term) := 
+  Let PTyEq (wl : wfLCon) (Γ : context) (A B : term) := True.
+  Let PTyRedEq (wl : wfLCon) (Γ : context) (A B : term) := 
     isType A × isType B.
-  Let PNeEq (Γ : context) (A t u : term) := 
+  Let PNeEq (wl : wfLCon) (Γ : context) (A t u : term) := 
     whne t × whne u.
-  Let PNeRedEq (Γ : context) (A t u : term) :=
-    [× whne t, whne u & isType A].
-  Let PTmEq (Γ : context) (A t u : term) := True.
-  Let PTmRedEq (Γ : context) (A t u : term) := 
+  Let PNeRedEq (wl : wfLCon) (Γ : context) (A t u : term) :=
+    [× whne t, whne u & whnf A].
+  Let PTmEq (wl : wfLCon) (Γ : context) (A t u : term) := True.
+  Let PTmRedEq (wl : wfLCon) (Γ : context) (A t u : term) := 
     [× whnf t, whnf u & isType A].
 
-  Theorem algo_conv_wh :
-    AlgoConvInductionConcl PTyEq PTyRedEq PNeEq PNeRedEq PTmEq PTmRedEq.
+  Theorem algo_conv_wh (wl : wfLCon) :
+    AlgoConvInductionConcl PTyEq PTyRedEq PNeEq PNeRedEq PTmEq PTmRedEq wl.
   Proof.
     subst PTyEq PTyRedEq PNeEq PNeRedEq PTmEq PTmRedEq; cbn.
     apply AlgoConvInduction.
     all: intros ; prod_splitter ; prod_hyp_splitter.
     all: try solve [now constructor].
-    all: gen_typing. 
+    all: now gen_typing.
   Qed.
 End AlgTypingWh.
+
+
+(** ** Determinism: there is at most one inferred type *)
+
+Section AlgoTypingDet.
+
+Import AlgorithmicTypingData.
+
+Let PTyEq (wl : wfLCon) (Γ : context) (A B : term) := True.
+Let PTyRedEq (wl : wfLCon) (Γ : context) (A B : term) := True.
+Let PNeEq (wl : wfLCon) (Γ : context) (A t u : term) := 
+  forall A' u', [Γ |-[al] t ~ u' ▹ A']< wl > -> A' = A.
+Let PNeRedEq (wl : wfLCon) (Γ : context) (A t u : term) :=
+  forall A' u', [Γ |-[al] t ~h u' ▹ A']< wl > -> A' = A.
+Let PTmEq (wl : wfLCon) (Γ : context) (A t u : term) := True.
+Let PTmRedEq (wl : wfLCon) (Γ : context) (A t u : term) := True.
+
+Theorem algo_conv_det (wl : wfLCon) :
+  AlgoConvInductionConcl PTyEq PTyRedEq PNeEq PNeRedEq PTmEq PTmRedEq wl.
+Proof.
+  subst PTyEq PTyRedEq PNeEq PNeRedEq PTmEq PTmRedEq; cbn.
+  apply AlgoConvInduction.
+  all: try easy.
+  - intros * ? * Hconv.
+    inversion Hconv ; subst ; clear Hconv.
+    now eapply in_ctx_inj.
+  - intros * ? IH ? ? ?? Hconv.
+    inversion Hconv ; subst ; clear Hconv ; refold.
+    apply IH in H6.
+    now inversion H6.
+  - intros * ? IH ?????? ?? Hconv.
+    inversion Hconv ; subst ; clear Hconv ; refold.
+    now reflexivity.
+  - intros * ? IH ?????? ?? Hconv.
+    inversion Hconv ; subst ; clear Hconv ; refold.
+    now reflexivity.
+  - intros * ? IH ?? ?? Hconv.
+    inversion Hconv ; subst ; clear Hconv ; refold.
+    now reflexivity.
+  - intros * ? IH ?? Hconv.
+    inversion Hconv; subst; clear Hconv; refold.
+    apply IH in H3.
+    now inversion H3.
+  - intros * ? IH ?? Hconv.
+    inversion Hconv; subst; clear Hconv; refold.
+    apply IH in H3.
+    now inversion H3.
+  - intros * ? IH (*? _ ? _ ? _*) ? _ ? _ ? _ ? _ ? _ * Hconv.
+    inversion Hconv; now subst.
+  - intros * ? IH ? ?  Hconv.
+    inversion Hconv ; subst ; clear Hconv ; refold.
+    reflexivity.
+  - intros * ? IH ???? Hconv.
+    inversion Hconv ; subst ; clear Hconv ; refold.
+    eapply IH in H2 as ->.
+    eapply whred_det ; eauto.
+    all: now eapply isType_whnf.
+Qed.
+
+Theorem algo_typing_det (wl : wfLCon) :
+  AlgoTypingInductionConcl wl
+    (fun _ _ => True)
+    (fun Γ A t => forall A', [Γ |-[al] t ▹ A']< wl > -> A' = A)
+    (fun Γ A t => whnf A -> forall A', whnf A' -> [Γ |-[al] t ▹h A']< wl > -> A' = A)
+    (fun _ _ _ => True).
+Proof.
+  apply AlgoTypingInduction.
+  all: try easy.
+  - intros * ? ? Hinf.
+    inversion Hinf ; subst ; clear Hinf.
+    now eapply in_ctx_inj.
+  - intros * ? IHA ? IHB ? Hconv.
+    now inversion Hconv.
+  - intros * ?? ? IHt ? Hconv.
+    inversion Hconv ; subst ; clear Hconv ; refold.
+    eapply IHt in H7 ; subst.
+    now reflexivity.
+  - intros * ? IHf ?? ? Hconv.
+    inversion Hconv ; subst ; clear Hconv ; refold.
+    eapply IHf in H6.
+    2-3:gen_typing.
+    now inversion H6.
+  - intros * Hconv.
+    now inversion Hconv.
+  - intros * Hconv.
+    now inversion Hconv.
+  - intros * ?? ? Hconv.
+    now inversion Hconv.
+  - intros * ? IH ?????? ? Hconv.
+    now inversion Hconv.
+  - intros * Hconv.
+    now inversion Hconv.
+  - intros * Hconv.
+    now inversion Hconv.
+  - intros * Hconv.
+    now inversion Hconv.
+  - intros * ? IH ? Hconv.
+    now inversion Hconv.
+  - intros * ? IH ??????? Hconv.
+    now inversion Hconv.
+  - intros * Hconv.
+    now inversion Hconv.
+  - intros * ? IH ?? ? Hconv.
+    now inversion Hconv.
+  - intros * ? IH ??? Hconv.
+    now inversion Hconv.
+  - intros * ????????? Hconv.
+    now inversion Hconv.
+  - intros * ? IH ? Hconv.
+    inversion Hconv; subst; refold.
+    apply IH in H3; try constructor.
+    now inversion H3.
+  - intros * ? IH ? Hconv.
+    inversion Hconv; subst; refold.
+    apply IH in H3; try constructor.
+    now inversion H3.
+  - intros * ?????? * Hconv; inversion Hconv; now subst.
+  - intros * ???? * Hconv; now inversion Hconv.
+  - intros * ???????????? * Hconv; now inversion Hconv.
+  - intros * ? IH ?? ?? Hconv.
+    inversion Hconv ; subst ; clear Hconv ; refold.
+    eapply IH in H3 ; subst.
+    now eapply whred_det.
+Qed.
+
+End AlgoTypingDet.
